theories/logrel/logrel_prim.v
@@ -13,8 +13,8 @@ Section logrel_prim.
   Definition trans_rel_primary (i:VMID) (trans trans': gmap Word transaction): Prop :=
    map_Forall (λ h tran,
           ((tran.1.1.1.1 ≠ i ∧ tran.1.1.1.2 ≠ i) -> ∃ tran', trans' !! h = Some tran' ∧ tran = tran') ∧
-          ((tran.1.1.1.1 = i ∧ tran.2 = true) -> ∃ tran', trans' !! h = Some tran' ∧ tran = tran') ∧
-          ((tran.1.1.1.2= i ∧ tran.1.2 ≠ Donation) -> ∃ tran', trans' !! h = Some tran' ∧ tran.1 = tran'.1)
+          ((tran.1.1.1.2 = V0 ∧ tran.2 = true) -> ∃ tran', trans' !! h = Some tran' ∧ tran = tran') ∧
+          ((tran.1.1.1.1 = V0 ∧ tran.1.2 ≠ Donation) -> ∃ tran', trans' !! h = Some tran' ∧ tran.1 = tran'.1)
      ) trans.
 
   Definition transaction_pagetable_entries_transferred_all (trans: gmap Addr transaction) : iProp Σ:=
@@ -25,16 +25,28 @@ Section logrel_prim.
     (big_sepFM trans (λ kv, kv.2.2 = false) (λ k v, k -{1/4}>t v.1 ∗ k -{1/2}>re v.2)%I).
 
   Definition transaction_pagetable_entries_transferred_except (i: VMID) (trans: gmap Addr transaction) : iProp Σ:=
-    big_sepFM trans (λ kv, kv.2.1.2 = Donation ∧ ¬(kv.2.1.1.1.2 = i ∨ kv.2.1.1.1.1 = i)) (λ k v, k -{1/4}>t v.1 ∗ pgt_1_4 v.1.1.2 v.1.1.1.1 true)%I.
+    big_sepFM trans (λ kv, kv.2.1.2 = Donation ∧ ¬(kv.2.1.1.1.1 = i ∨ kv.2.1.1.1.2 = i)) (λ k v, k -{1/4}>t v.1 ∗ pgt_1_4 v.1.1.2 v.1.1.1.1 true)%I.
 
   Definition retrievable_transaction_transferred_except (i: VMID) (trans: gmap Addr transaction) : iProp Σ:=
-    (big_sepFM trans (λ kv, ¬(kv.2.1.1.1.2 = i ∨ kv.2.1.1.1.1 = i)) (λ k v, k -{1/2}>re v.2 )%I) ∗
-    (big_sepFM trans (λ kv, ¬(kv.2.1.1.1.2 = i ∨ kv.2.1.1.1.1 = i) ∧ kv.2.2 = false) (λ k v, k -{1/4}>t v.1 ∗ k -{1/2}>re v.2)%I).
+    (big_sepFM trans (λ kv, ¬(kv.2.1.1.1.1 = i ∨ kv.2.1.1.1.2 = i)) (λ k v, k -{1/2}>re v.2 )%I) ∗
+    (big_sepFM trans (λ kv, ¬(kv.2.1.1.1.1 = i ∨ kv.2.1.1.1.2 = i) ∧ kv.2.2 = false) (λ k v, k -{1/4}>t v.1 ∗ k -{1/2}>re v.2)%I).
 
   Definition transferred_memory_pages_all (trans : gmap Word transaction) :=
     pages_in_trans (filter (λ kv, ¬(kv.2.2 = true ∧ kv.2.1.2 = Lending)) trans).
 
-  Program Definition interp_access_prim p_tx p_rx ps_acc trans: iPropO Σ:=
+  Definition transferred_memory_pages_slice (j: VMID) (i:VMID) (trans : gmap Addr transaction) :=
+    pages_in_trans (filter (λ kv, (kv.2.1.1.1.1 = i ∧ kv.2.1.1.1.2 = j) ∧ ¬(kv.2.2 = true ∧ kv.2.1.2 = Lending)) trans).
+
+  Definition retrievable_transaction_transferred_slice (i:VMID) (j: VMID) (trans : gmap Addr transaction) : iProp Σ :=
+    (big_sepFM trans (λ kv, kv.2.1.1.1.1 = i ∧ kv.2.1.1.1.2 = j) (λ k v, k -{1/2}>re v.2 )%I) ∗
+    (big_sepFM trans (λ kv, (kv.2.1.1.1.1 = i ∧ kv.2.1.1.1.2 = j) ∧ kv.2.2 = false) (λ k v, k -{1/4}>t v.1 ∗ k -{1/2}>re v.2)%I).
+
+  Definition transaction_pagetable_entries_transferred_slice (i: VMID) (j: VMID) (trans: gmap Addr transaction) : iProp Σ :=
+    big_sepFM trans (λ kv, (kv.2.1.1.1.1 = i ∧ kv.2.1.1.1.2 = j) ∧ kv.2.1.2 = Donation ) (λ k v, k -{1/4}>t v.1 ∗ pgt_1_4 v.1.1.2 v.1.1.1.1 true)%I.
+
+  Definition set_of_vmids : gset VMID := (list_to_set list_of_vmids).
+
+  Program Definition interp_access_prim p_tx p_rx ps_acc trans (Φ: (gmap Addr transaction) -> (VMID * VMID)-> iProp Σ): iPropO Σ:=
     (
       let ps_macc_trans := (transferred_memory_pages_all trans) in
       let ps_oea := ps_acc ∖ {[p_rx;p_tx]} ∖ (currently_accessible_in_trans_memory_pages V0 trans) in
@@ -50,11 +62,12 @@ Section logrel_prim.
       (* transferred *)
       (∃ rx_state, RX_state@ V0 := rx_state) ∗ (rx_page V0 p_rx) ∗ (∃ mem_rx, memory_page p_rx mem_rx) ∗
       transaction_hpool_global_transferred trans ∗
+      rx_pages (list_to_set (list_of_vmids) ∖ {[V0]}) ∗
+      ([∗ set] i ∈ set_of_vmids, [∗ set] j ∈ set_of_vmids, Φ trans (i,j)) ∗
       transaction_pagetable_entries_transferred_all trans ∗
       retrievable_transaction_transferred_all trans ∗
       (∃ mem_trans, memory_pages ps_macc_trans mem_trans) ∗
-      rx_pages (list_to_set (list_of_vmids) ∖ {[V0]}) ∗
-      [∗ set] i ∈ list_to_set (list_of_vmids) ∖ {[V0]}, VMProp (i:VMID) (vmprop_unknown i p_tx p_rx) (1/2)%Qp
+      [∗ set] i ∈ set_of_vmids ∖ {[V0]}, VMProp (i:VMID) (vmprop_unknown i p_tx p_rx) (1/2)%Qp
     )%I.
 
 End logrel_prim.
