theories/logrel/logrel_prim_extra.v
@@ -2,7 +2,7 @@ From iris.proofmode Require Import tactics.
 From machine_program_logic.program_logic Require Import weakestpre.
 From HypVeri.lang Require Import lang.
 From HypVeri.algebra Require Import base base_extra mem pagetable trans.
-From HypVeri.logrel Require Import logrel_prim.
+From HypVeri.logrel Require Import logrel_prim big_sepSS.
 From HypVeri Require Import proofmode.
 From stdpp Require fin_map_dom.
 Import uPred.
@@ -13,44 +13,196 @@ Section logrel_prim_extra.
   Context `{vmG: !gen_VMG Σ}.
 
   (* Lemmas about relationships between transferred_all, transferred, and transferred_except *)
-  Lemma transaction_pagetable_entries_transferred_split i trans:
-    transaction_pagetable_entries_transferred_all trans ⊣⊢ transaction_pagetable_entries_transferred i trans ∗
-                                                 transaction_pagetable_entries_transferred_except i trans.
-  Proof. iApply (big_sepFM_split_decide). Qed.
+  (* Lemma transaction_pagetable_entries_transferred_split i trans: *)
+  (*   transaction_pagetable_entries_transferred_all trans ⊣⊢ transaction_pagetable_entries_transferred i trans ∗ *)
+  (*                                                transaction_pagetable_entries_transferred_except i trans. *)
+  (* Proof. iApply (big_sepFM_split_decide). Qed. *)
 
-  Lemma retrievable_transaction_transferred_split i trans:
-   retrievable_transaction_transferred_all trans ⊣⊢ retrievable_transaction_transferred i trans ∗
-                                                 retrievable_transaction_transferred_except i trans.
+  (* Lemma retrievable_transaction_transferred_split i trans: *)
+  (*  retrievable_transaction_transferred_all trans ⊣⊢ retrievable_transaction_transferred i trans ∗ *)
+  (*                                                retrievable_transaction_transferred_except i trans. *)
+  (* Proof. *)
+  (*   rewrite /retrievable_transaction_transferred /retrievable_transaction_transferred_all /retrievable_transaction_transferred_except. *)
+  (*   iSplit. *)
+  (*   iIntros "(H1 & H2)". *)
+  (*   iDestruct (big_sepFM_split_decide (Q:= (λ kv, kv.2.1.1.1.2 = i ∨ kv.2.1.1.1.1 = i)) with "H1") as "[H11 H12]". *)
+  (*   rewrite (big_sepFM_iff (Q:= (λ kv, kv.2.1.1.1.2 = i ∨ kv.2.1.1.1.1 = i))). iFrame "H11". *)
+  (*   rewrite (big_sepFM_iff (Q:= (λ kv, ¬ (kv.2.1.1.1.2 = i ∨ kv.2.1.1.1.1 = i)))). iFrame "H12". *)
+  (*   iDestruct (big_sepFM_split_decide (Q:= (λ kv, kv.2.1.1.1.1 = i ∨ kv.2.1.1.1.2 = i)) with "H2") as "[H21 H22]". *)
+  (*   iSplitL "H21". *)
+  (*   iApply (big_sepFM_iff with "H21"). intros. split;intros [? ?];auto. *)
+  (*   iApply (big_sepFM_iff with "H22"). intros. split;intros [? ?];split;auto. intro Hor;apply H;destruct Hor;eauto. *)
+  (*   intro Hor;apply H0;destruct Hor;eauto. *)
+  (*   intros. split;intros H;eauto. destruct H;done. *)
+  (*   intros. split;intros H;eauto. destruct H;done. *)
+  (*   iIntros "([H11 H12] & [H21 H22])". *)
+  (*   iSplitL "H11 H21". *)
+  (*   iApply (big_sepFM_split_decide (Q:= (λ kv, kv.2.1.1.1.2 = i ∨ kv.2.1.1.1.1 = i))). *)
+  (*   rewrite (big_sepFM_iff (Q:= (λ kv, kv.2.1.1.1.2 = i ∨ kv.2.1.1.1.1 = i))). iFrame "H11". *)
+  (*   rewrite (big_sepFM_iff (Q:= (λ kv, ¬ (kv.2.1.1.1.2 = i ∨ kv.2.1.1.1.1 = i)))). iFrame "H21". *)
+  (*   intros. split;intros H;eauto. destruct H;done. *)
+  (*   intros. split;intros H;eauto. destruct H;done. *)
+  (*   iApply (big_sepFM_split_decide (Q:= (λ kv, kv.2.1.1.1.1 = i ∨ kv.2.1.1.1.2 = i))). *)
+  (*   iSplitL "H12". *)
+  (*   iApply big_sepFM_iff. 2: iFrame "H12". *)
+  (*   intros. split;intros H;eauto. destruct H;auto. destruct H;split;auto. *)
+  (*   iApply big_sepFM_iff. 2: iFrame "H22". *)
+  (*   intros. split;intros H;eauto. destruct H as [? H];split;auto. *)
+  (*   intro. apply H. destruct H1;auto. *)
+  (*   destruct H as [? H];split;auto. *)
+  (*   intro. apply H0. destruct H1;auto. *)
+  (* Qed. *)
+
+  Lemma big_sepFM_trans_split i (trans: gmap Addr transaction) `{∀ x, Decision (Q x)} (Φ: _ -> _ -> iPropO Σ):
+    map_Forall (λ k (v:transaction), v.1.1.1.1 ≠ v.1.1.1.2) trans ->
+    big_sepFM trans (λ kv : Addr * transaction, ((kv.2.1.1.1.1 = i ∨ kv.2.1.1.1.2 = i) ∧ (Q kv))%type) Φ
+    ⊣⊢
+    (big_sepFM trans (λ kv : Addr * transaction, (kv.2.1.1.1.1 = i ∧ (Q kv))%type) Φ ∗
+     big_sepFM trans (λ kv : Addr * transaction, (kv.2.1.1.1.2 = i ∧ (Q kv))%type) Φ).
   Proof.
-    rewrite /retrievable_transaction_transferred /retrievable_transaction_transferred_all /retrievable_transaction_transferred_except.
-    iSplit.
-    iIntros "(H1 & H2)".
-    iDestruct (big_sepFM_split_decide (Q:= (λ kv, kv.2.1.1.1.2 = i ∨ kv.2.1.1.1.1 = i)) with "H1") as "[H11 H12]".
-    rewrite (big_sepFM_iff (Q:= (λ kv, kv.2.1.1.1.2 = i ∨ kv.2.1.1.1.1 = i))). iFrame "H11".
-    rewrite (big_sepFM_iff (Q:= (λ kv, ¬ (kv.2.1.1.1.2 = i ∨ kv.2.1.1.1.1 = i)))). iFrame "H12".
-    iDestruct (big_sepFM_split_decide (Q:= (λ kv, kv.2.1.1.1.1 = i ∨ kv.2.1.1.1.2 = i)) with "H2") as "[H21 H22]".
-    iSplitL "H21".
-    iApply (big_sepFM_iff with "H21"). intros. split;intros [? ?];auto.
-    iApply (big_sepFM_iff with "H22"). intros. split;intros [? ?];split;auto. intro Hor;apply H;destruct Hor;eauto.
-    intro Hor;apply H0;destruct Hor;eauto.
-    intros. split;intros H;eauto. destruct H;done.
-    intros. split;intros H;eauto. destruct H;done.
-    iIntros "([H11 H12] & [H21 H22])".
-    iSplitL "H11 H21".
-    iApply (big_sepFM_split_decide (Q:= (λ kv, kv.2.1.1.1.2 = i ∨ kv.2.1.1.1.1 = i))).
-    rewrite (big_sepFM_iff (Q:= (λ kv, kv.2.1.1.1.2 = i ∨ kv.2.1.1.1.1 = i))). iFrame "H11".
-    rewrite (big_sepFM_iff (Q:= (λ kv, ¬ (kv.2.1.1.1.2 = i ∨ kv.2.1.1.1.1 = i)))). iFrame "H21".
-    intros. split;intros H;eauto. destruct H;done.
-    intros. split;intros H;eauto. destruct H;done.
-    iApply (big_sepFM_split_decide (Q:= (λ kv, kv.2.1.1.1.1 = i ∨ kv.2.1.1.1.2 = i))).
-    iSplitL "H12".
-    iApply big_sepFM_iff. 2: iFrame "H12".
-    intros. split;intros H;eauto. destruct H;auto. destruct H;split;auto.
-    iApply big_sepFM_iff. 2: iFrame "H22".
-    intros. split;intros H;eauto. destruct H as [? H];split;auto.
-    intro. apply H. destruct H1;auto.
-    destruct H as [? H];split;auto.
-    intro. apply H0. destruct H1;auto.
+    intros Hfalse.
+    rewrite -big_sepFM_split_lor_weak.
+    2:{ intros ? ? ? [[? _ ] [? _]].
+        eapply (Hfalse);eauto.
+        rewrite H1 H2 //.
+    }
+    apply big_sepFM_iff.
+    intros. split.
+    intros [[|] ];eauto.
+    intros [[]|[]];eauto.
   Qed.
+
+  Lemma elem_of_set_of_vmids i:
+    i ∈ set_of_vmids.
+  Proof.
+    rewrite /set_of_vmids.
+    rewrite elem_of_list_to_set.
+    rewrite elem_of_list_In.
+    apply in_list_of_vmids.
+  Qed.
+
+  Lemma big_sepFM_big_sepS_trans_sndr i (trans: gmap Addr transaction) `{∀ x, Decision (Q x)} (Φ: _ -> _ -> iPropO Σ):
+  ([∗ set] y ∈ set_of_vmids,  big_sepFM trans (λ kv : Addr * transaction, (kv.2.1.1.1.1 = i ∧ kv.2.1.1.1.2 = y ∧ Q kv)%type) Φ)
+  ⊣⊢ big_sepFM trans (λ kv : Addr * transaction, (kv.2.1.1.1.1 = i ∧ Q kv)%type) Φ.
+  Proof.
+    rewrite (big_sepFM_iff (Q:= (λ kv, kv.2.1.1.1.1 = i ∧ kv.2.1.1.1.2 ∈ set_of_vmids ∧ Q kv))).
+    2:{
+      intros. split.
+      intros []. split;auto;split;auto. apply elem_of_set_of_vmids.
+      intros [? []]. split;done.
+    }
+    iInduction set_of_vmids as [|x s Hin] "IH" using set_ind_L.
+    {
+      iSplit; iIntros.
+      iApply big_sepFM_False.
+      intros ? [_ [? _]].
+      set_solver.
+      by iApply big_sepS_empty.
+    }
+    {
+      rewrite big_sepS_union //.
+      2: set_solver+ Hin.
+      rewrite big_sepS_singleton.
+      rewrite (big_sepFM_iff
+                 (P:= (λ kv , (kv.2.1.1.1.1 = i ∧ kv.2.1.1.1.2 ∈ {[x]} ∪ s ∧ Q kv)))
+                 (Q:= (λ kv, (kv.2.1.1.1.1 = i ∧ kv.2.1.1.1.2 = x ∧ Q kv ∨ kv.2.1.1.1.1 = i ∧ kv.2.1.1.1.2 ∈ s ∧ Q kv )%type))).
+      2:{
+        intros kv. rewrite elem_of_union. split.
+        intros [? [[|] ?]]. left;split;auto;split;auto. set_solver.
+        right;split;auto.
+        intros [[? []]|[?[]]];split;auto;split;auto.
+        left;set_solver.
+      }
+      rewrite big_sepFM_split_lor.
+      2:{ intros ? (?&?&?&?). set_solver. }
+      iSplit;iIntros "[$ ?]"; by iApply "IH".
+    }
+  Qed.
+
+  Lemma big_sepFM_big_sepS_trans_rcvr i (trans: gmap Addr transaction) `{∀ x, Decision (Q x)} (Φ: _ -> _ -> iPropO Σ):
+  ([∗ set] y ∈ set_of_vmids,  big_sepFM trans (λ kv : Addr * transaction, (kv.2.1.1.1.1 = y ∧ kv.2.1.1.1.2 = i ∧ Q kv)%type) Φ)
+  ⊣⊢ big_sepFM trans (λ kv : Addr * transaction, (kv.2.1.1.1.2 = i ∧ Q kv)%type) Φ.
+  Proof.
+    rewrite (big_sepFM_iff (Q:= (λ kv, kv.2.1.1.1.1 ∈ set_of_vmids ∧ kv.2.1.1.1.2 = i ∧ Q kv))).
+    2:{
+      intros. split.
+      intros []. split;auto. apply elem_of_set_of_vmids.
+      intros [? []]. split;done.
+    }
+    iInduction set_of_vmids as [|x s Hin] "IH" using set_ind_L.
+    {
+      iSplit; iIntros.
+      iApply big_sepFM_False.
+      intros ? [? _]. set_solver.
+      by iApply big_sepS_empty.
+    }
+    {
+      rewrite big_sepS_union //.
+      2: set_solver+ Hin.
+      rewrite big_sepS_singleton.
+      rewrite (big_sepFM_iff
+                 (P:= (λ kv , (kv.2.1.1.1.1 ∈ {[x]} ∪ s ∧ kv.2.1.1.1.2 = i ∧ Q kv)))
+                 (Q:= (λ kv, (kv.2.1.1.1.1 = x ∧ kv.2.1.1.1.2 = i ∧ Q kv ∨ kv.2.1.1.1.1 ∈ s ∧ kv.2.1.1.1.2 = i ∧ Q kv )%type))).
+      2:{
+        intros kv. rewrite elem_of_union. split.
+        intros [[|] [? ?]]. left;split;auto. set_solver.
+        right;split;auto.
+        intros [[? []]|[?[]]];split;auto.
+        left;set_solver.
+      }
+      rewrite big_sepFM_split_lor.
+      2:{ intros ? (?&?&?&?). set_solver. }
+      iSplit;iIntros "[$ ?]"; by iApply "IH".
+    }
+  Qed.
+
+  Lemma transaction_pagetable_entries_transferred_equiv i (trans: gmap Addr transaction):
+    map_Forall (λ k (v:transaction), v.1.1.1.1 ≠ v.1.1.1.2) trans ->
+    big_sepSS_singleton set_of_vmids i (λ ij, transaction_pagetable_entries_transferred_slice ij.1 ij.2 trans) ⊣⊢
+      transaction_pagetable_entries_transferred i trans.
+  Proof.
+    intros Hfalse.
+    rewrite /transaction_pagetable_entries_transferred.
+    rewrite (big_sepFM_iff (Q:= (λ kv : Addr * transaction,((kv.2.1.1.1.1 = i ∨ kv.2.1.1.1.2 = i) ∧ kv.2.1.2 = Donation)%type))).
+    2:{  intros. split; intros [? ?];done. }
+    rewrite big_sepFM_trans_split //.
+    rewrite /big_sepSS_singleton.
+    rewrite big_sepS_sep /=.
+    rewrite /transaction_pagetable_entries_transferred_slice.
+    iSplit.
+    iIntros "[H1 H2]";iSplitL "H1";first iApply big_sepFM_big_sepS_trans_sndr.
+    iApply big_sepS_proper.
+    2: iExact "H1".
+    intros. iApply big_sepFM_iff.
+    intros. split;intros [[] []];split;eauto.
+    iApply big_sepFM_big_sepS_trans_rcvr.
+    iApply big_sepS_proper.
+    2: iExact "H2".
+    intros. iApply big_sepFM_iff.
+    intros. split;intros [[] []];split;eauto.
+    iIntros "[H1 H2]";iSplitL "H1".
+    iDestruct (big_sepFM_big_sepS_trans_sndr with "H1") as "H1".
+    iApply big_sepS_proper.
+    2: iExact "H1".
+    intros. iApply big_sepFM_iff.
+    intros. split;intros [[] []];split;eauto.
+    iDestruct (big_sepFM_big_sepS_trans_rcvr with "H2") as "H2".
+    iApply big_sepS_proper.
+    2: iExact "H2".
+    intros. iApply big_sepFM_iff.
+    intros. split;intros [[] []];split;eauto.
+   Qed.
+
+  Lemma retrievable_transaction_transferred_equiv i (trans: gmap Addr transaction):
+    big_sepSS_singleton set_of_vmids i (λ ij, retrievable_transaction_transferred_to ij.2 ij.1 trans) ⊣⊢
+    retrievable_transaction_transferred i trans.
+  Proof.
+  Admitted.
+
+  Lemma transferred_memory_pages_equiv i (trans: gmap Addr transaction):
+    big_sepSS_singleton set_of_vmids i (λ ij, ∃mem, memory_pages (transferred_memory_pages_to ij.2 ij.1 trans) mem) ⊣⊢
+    ∃mem, memory_pages (transferred_memory_pages i trans) mem.
+  Proof.
+  Admitted.
 
 End logrel_prim_extra.
